LeanSubst/Types/Option.lean
@@ -1,51 +1,52 @@
 
--- import LeanSubst.Laws
+import LeanSubst.Class
 
 namespace LeanSubst
 
 universe u1 u2 u3
-variable {S : Type u1} {T : Type u2} {U : Type u3}
+variable {S : Type u1} {T T1 T2 : Type u2} {U : Type u3}
+variable {V : List (Type u2)}
 
--- def Option.rmap [i : RenMap S T] (r : Ren T) : Option S -> Option S
--- | none => none
--- | some t => some t⟨r⟩
+def Option.rmap [RenMap S V] (r : RenVec V) : Option S -> Option S
+| none => none
+| some t => some t⟨r,⟩
 
--- instance [RenMap S T] : RenMap (Option S) T where
---   rmap := Option.rmap
+instance [RenMap S V] : RenMap (Option S) V where
+  rmap := Option.rmap
 
--- @[simp, grind =]
--- theorem Option.rmap_none [RenMap S T] {r : Ren T} : (@Option.none S)⟨r⟩ = none := by
---   simp [RenMap.rmap, Option.rmap]
+@[simp, grind =]
+theorem Option.rmap_none [RenMap S V] {r : RenVec V} : (@Option.none S)⟨r,⟩ = none := by
+  simp [RenMap.rmap, Option.rmap]
 
--- @[simp, grind =]
--- theorem Option.rmap_some [RenMap S T] {x : S} {r : Ren T} : (some x)⟨r⟩ = some x⟨r⟩ := by
---   simp [RenMap.rmap, Option.rmap]
+@[simp, grind =]
+theorem Option.rmap_some [RenMap S V] {x : S} {r : RenVec V} : (some x)⟨r,⟩ = some x⟨r,⟩ := by
+  simp [RenMap.rmap, Option.rmap]
 
--- instance [RenMap S T] [RenMapId S T] : RenMapId (Option S) T where
---   apply_id := by intro t; cases t <;> simp
+instance [RenMap S V] [RenMapId S V] : RenMapId (Option S) V where
+  apply_id := by intro t; cases t <;> simp
 
--- instance [RenMap S T] [RenMapCompose S T] : RenMapCompose (Option S) T where
---   apply_compose := by intro s σ τ; cases s <;> simp
+instance [RenMap S V] [RenMapCompose S V] : RenMapCompose (Option S) V where
+  apply_compose := by intro s σ τ; cases s <;> simp
 
--- def Option.smap [SubstMap S T] (σ : Subst T) : Option S -> Option S
--- | none => none
--- | some t => some t[σ]
+def Option.smap [SubstMap S V] (σ : SubstVec V) : Option S -> Option S
+| none => none
+| some t => some t[σ,]
 
--- instance [SubstMap S T] : SubstMap (Option S) T where
---   smap := Option.smap
+instance [SubstMap S V] : SubstMap (Option S) V where
+  smap := Option.smap
 
--- @[simp, grind =]
--- theorem Option.smap_none [SubstMap S T] {σ : Subst T} : (@Option.none S)[σ] = none := by
---   simp [SubstMap.smap, Option.smap]
+@[simp, grind =]
+theorem Option.smap_none [SubstMap S V] {σ : SubstVec V} : (@Option.none S)[σ,] = none := by
+  simp [SubstMap.smap, Option.smap]
 
--- @[simp, grind =]
--- theorem Option.smap_some [SubstMap S T] {x : S} {σ : Subst T} : (some x)[σ] = some x[σ] := by
---   simp [SubstMap.smap, Option.smap]
+@[simp, grind =]
+theorem Option.smap_some [SubstMap S V] {x : S} {σ : SubstVec V} : (some x)[σ,] = some x[σ,] := by
+  simp [SubstMap.smap, Option.smap]
 
--- instance [RenMap S T] [SubstMap S T] [SubstMapId S T] : SubstMapId (Option S) T where
---   apply_id := by intro t; cases t <;> simp
+instance [RenMap S V] [SubstMap S V] [SubstMapId S V] : SubstMapId (Option S) V where
+  apply_id := by intro t; cases t <;> simp
 
--- instance [SubstMap T T] [SubstMap S T] [SubstMapCompose S T] : SubstMapCompose (Option S) T where
---   apply_compose := by intro s σ τ; cases s <;> simp
+instance [SubstMapAll V] [SubstMap S V] [SubstMapCompose S V] : SubstMapCompose (Option S) V where
+  apply_compose := by intro s σ τ; cases s <;> simp
 
 end LeanSubst
