Examples/SystemFWithNat/Theory.lean
@@ -1,0 +1,149 @@
+
+import Examples.SystemFWithNat.Term
+open LeanSubst
+
+namespace SystemFWithNat
+
+inductive Kinding : List Unit -> Ty -> Prop where
+| var {Δ x} :
+  Δ[x]? = some .unit ->
+  Kinding Δ (.var x)
+| nat {Δ} :
+  Kinding Δ .nat
+| arrow {Δ A B} :
+  Kinding Δ A ->
+  Kinding Δ B ->
+  Kinding Δ (.arrow A B)
+| all {Δ P} :
+  Kinding (.unit::Δ) P ->
+  Kinding Δ (.all P)
+
+notation:170 Δ:170 " ⊢ " A:170 " type" => Kinding Δ A
+
+inductive Typing  : List Unit -> List Ty -> Term -> Ty -> Prop where
+| var {Δ Γ x A} :
+  Γ[x]? = some A ->
+  Δ ⊢ A type ->
+  Typing Δ Γ (.var x) A
+| app {Δ Γ A B f a} :
+  Typing Δ Γ f (.arrow A B) ->
+  Typing Δ Γ a A ->
+  Typing Δ Γ (.app f a) B
+| lam {Δ Γ A B t} :
+  Δ ⊢ A type ->
+  Typing Δ (A::Γ) t B ->
+  Typing Δ Γ (.lam A t) (.arrow A B)
+| tapp {Δ Γ P P' A f} :
+  Typing Δ Γ f (.all P) ->
+  Δ ⊢ A type ->
+  P' = P[su A::𝐬0] ->
+  Typing Δ Γ (.tapp f A) P'
+| tlam {Δ Γ P t} :
+  Typing (.unit::Δ) Γ⟨𝐫1(Ty)⟩ t P ->
+  Typing Δ Γ (.tlam t) (.all P)
+| zero {Δ Γ} :
+  Typing Δ Γ .zero .nat
+| succ {Δ Γ n} :
+  Typing Δ Γ n .nat ->
+  Typing Δ Γ (.succ n) .nat
+| nrec {Δ Γ A z s n} :
+  Typing Δ Γ z A ->
+  Typing Δ (A::.nat::Γ) s A ->
+  Typing Δ Γ n .nat ->
+  Typing Δ Γ (.nrec z s n) A
+
+notation:200 Δ:200 "&" Γ:200 " ⊢ " t:200 " : " A:200 => Typing Δ Γ t A
+
+structure KindingRen (r : Ren Ty) (Δ Δ' : List Unit) where
+  act : ∀ {x T}, Δ[x]? = some T -> Δ'[r.act x]? = some T
+
+theorem KindingRen.succ {A X} : KindingRen (.succ Ty) X (A::X) := ⟨λ h => h⟩
+
+theorem KindingRen.lift {Δ Δ' : List Unit} (r : Ren Ty) (h : KindingRen r Δ Δ')
+  : KindingRen r.lift (.unit::Δ) (.unit::Δ')
+:= ⟨λ {x} _ j =>
+    match x with
+    | 0 => j
+    | _ + 1 => h.act j⟩
+
+theorem Kinding.rename {Δ Δ' A} {r : Ren Ty} (m : KindingRen r Δ Δ') : Δ ⊢ A type -> Δ' ⊢ A⟨r⟩ type
+| var j => var (m.act j)
+| nat => nat
+| arrow j1 j2 => arrow (j1.rename m) (j2.rename m)
+| all j => all (j.rename $ m.lift)
+
+structure KindingSubst (σ : Subst Ty) (Δ Δ' : List Unit) where
+  act : ∀ {x : Nat} {T}, Δ[x]? = some T -> Δ' ⊢ σ.act x type
+
+theorem KindingSubst.lift {Δ Δ' : List Unit} {σ : Subst Ty} (m : KindingSubst σ Δ Δ')
+  : KindingSubst σ.lift (.unit::Δ) (.unit::Δ')
+:= ⟨λ {x} _ j =>
+    match x with
+    | 0 => .var j
+    | _ + 1 =>
+      have lem := (m.act j).rename (Δ' := .unit::Δ') KindingRen.succ
+      by simp at lem; exact lem⟩
+
+theorem Kinding.subst {Δ Δ' A} {σ : Subst Ty} (m : KindingSubst σ Δ Δ') : Δ ⊢ A type -> Δ' ⊢ A[σ] type
+| var j => m.act j
+| nat => nat
+| arrow j1 j2 => arrow (j1.subst m) (j2.subst m)
+| all j => all (j.subst $ m.lift)
+
+structure TypingRen (r : RenVec [Term, Ty]) (Δ Δ' : List Unit) (Γ Γ' : List Ty) where
+  act : (∀ {x T}, Δ[x]? = some T -> Δ'[r.2.1.act x]? = some T)
+    ∧ (∀ {x T} (ξ : Ren Ty), Γ⟨ξ⟩[x]? = some T -> Γ'⟨ξ⟩[r.1.act x]? = some T)
+
+theorem TypingRen.lift {Δ Δ' Γ Γ'} {r : RenVec [Term, Ty]} :
+  ∀ (_ : TypingRen r Δ Δ' Γ Γ') (U : List Unit) (T : List Ty),
+  TypingRen (r.lift [T.length, U.length])
+    (U ++ Δ) (U ++ Δ')
+    (T ++ Γ⟨Ren.add Ty U.length⟩) (T ++ Γ'⟨Ren.add Ty U.length⟩)
+| ⟨⟨act1, act2⟩⟩, U, T =>
+  ⟨⟨λ {x T'} j =>
+    match Nat.decLt x (U.length) with
+    | .isFalse h => by simp; grind
+    | .isTrue h => by simp; grind,
+    λ {x T'} (ξ : Ren Ty) j =>
+    match Nat.decLt x ((T⟨ξ⟩ : List Ty).length) with
+    | .isFalse h =>
+      have lem0 : T.length = (T⟨ξ⟩ : List Ty).length := by rw [List.rmap_length]
+      have lem1 : Γ'⟨Ren.add Ty U.length >> ξ⟩[r.1.act (x - T.length)]? = some T' := by
+        simp at j; rw [List.getElem?_append_right] at j; rw [<-lem0] at j
+        apply act2 (Ren.add Ty U.length >> ξ) j; grind
+      by {
+        simp; rw [lem0]; rw [Ren.lift_action_ge]
+        rw [List.getElem?_append_right]; simp
+        rw [<-lem0]; exact lem1
+        grind; grind
+      }
+    | .isTrue h => by {
+      have lem0 : T.length = (T⟨ξ⟩ : List Ty).length := by rw [List.rmap_length]
+      have lem1 : x < T.length := by grind
+      simp_all; grind
+    }⟩⟩
+
+theorem TypingRen.kind {Δ Δ' Γ Γ'} {r : RenVec [Term, Ty]}
+  : TypingRen r Δ Δ' Γ Γ' -> KindingRen r.2.1 Δ Δ'
+| ⟨act⟩ => ⟨act.1⟩
+
+theorem Typing.rename {Δ Δ' Γ Γ' A t} {r : RenVec [Term, Ty]} (m : TypingRen r Δ Δ' Γ Γ')
+  : Δ&Γ ⊢ t : A -> Δ'&Γ'⟨r.2.1⟩ ⊢ t⟨r,⟩ : A⟨r.2.1⟩
+| var (x := x) j1 j2 =>
+  have e := congr (f₁ := λ t => t⟨r.2.1⟩) rfl $ @m.act.2 x A 𝐫0 (j1 |> cast (by simp))
+  var (e |> cast (by simp)) (j2.rename m.kind)
+| app j1 j2 => app (j1.rename m) (j2.rename m)
+| lam (A := A) j1 j2 =>
+  have m' : TypingRen (r.lift [1, 0]) Δ Δ' (A::Γ) (A::Γ') := m.lift [] [A] |> cast (by simp)
+  lam (j1.rename m.kind) (j2.rename m')
+| tapp j1 j2 e => tapp (j1.rename m) (j2.rename m.kind) (by simp [e])
+| tlam j =>
+  have m' : TypingRen (r.lift [0, 1]) (()::Δ) (()::Δ') Γ⟨𝐫1(Ty)⟩ Γ'⟨𝐫1(Ty)⟩ := m.lift [.unit] []
+  tlam (j.rename m' |> cast (by simp; grind))
+| zero => zero
+| succ j => succ (j.rename m)
+| nrec j1 j2 j3 =>
+  have m' : TypingRen (r.lift [2, 0]) Δ Δ' (A::.nat::Γ) (A::.nat::Γ') := m.lift [] [A, .nat] |> cast (by simp)
+  nrec (j1.rename m) (j2.rename m') (j3.rename m)
+
+end SystemFWithNat
